pst API in elim pure

pulse/lib/steel/pulse/Pulse.Prover.ElimPure.fst
@@ -7,6 +7,8 @@ module T = FStar.Tactics.V2
 open FStar.List.Tot
 open Pulse.Syntax
 open Pulse.Checker.Pure
+open Pulse.Checker.VPropEquiv
+
 open Pulse.Typing
 module Metatheory = Pulse.Typing.Metatheory
 open Pulse.Reflection.Util
@@ -84,6 +86,15 @@ let mk (#g:env) (#v:vprop) (v_typing:tot_typing g v tm_vprop)
             elim_pure_typing g pp p_typing |)
   | _ -> None
 
+let elim_pure_frame (#g:env) (#ctxt:term) (#frame:term)
+  (ctxt_frame_typing:tot_typing g (ctxt * frame) tm_vprop)
+  (uvs:env { disjoint uvs g })
+  : T.Tac (g':env { env_extends g' g /\ disjoint uvs g' } &
+           ctxt':term &
+           tot_typing g' (ctxt' * frame) tm_vprop &
+           continuation_elaborator g (ctxt * frame) g' (ctxt' * frame)) =
+  add_elims is_elim_pure mk ctxt_frame_typing uvs
+
 let elim_pure (#g:env) (#ctxt:term) (ctxt_typing:tot_typing g ctxt tm_vprop)
   : T.Tac (g':env { env_extends g' g } &
            ctxt':term &
@@ -91,8 +102,51 @@ let elim_pure (#g:env) (#ctxt:term) (ctxt_typing:tot_typing g ctxt tm_vprop)
            continuation_elaborator g ctxt g' ctxt') =
   let ctxt_emp_typing : tot_typing g (tm_star ctxt tm_emp) tm_vprop = magic () in
   let (| g', ctxt', ctxt'_emp_typing, k |) =
-    add_elims is_elim_pure mk ctxt_emp_typing (mk_env (fstar_env g)) in
+    elim_pure_frame ctxt_emp_typing (mk_env (fstar_env g)) in
   let k = k_elab_equiv k (VE_Trans _ _ _ _ (VE_Comm _ _ _) (VE_Unit _ _))
                          (VE_Trans _ _ _ _ (VE_Comm _ _ _) (VE_Unit _ _)) in
   (| g', ctxt', star_typing_inversion_l ctxt'_emp_typing, k |)
  
+// a lot of this is copy-pasted from elim_exists_pst,
+//   can add a common function to Prover.Common
+let elim_pure_pst (#preamble:_) (pst:prover_state preamble)
+  : T.Tac (pst':prover_state preamble { pst' `pst_extends` pst }) =
+
+  let (| g', remaining_ctxt', ty, k |) =
+    elim_pure_frame
+      #pst.pg
+      #(list_as_vprop pst.remaining_ctxt)
+      #(preamble.frame * pst.ss.(pst.solved))
+      (magic ())
+      pst.uvs in
+
+  let k
+    : continuation_elaborator
+        pst.pg (list_as_vprop pst.remaining_ctxt * (preamble.frame * pst.ss.(pst.solved)))
+        g' (remaining_ctxt' * (preamble.frame * pst.ss.(pst.solved))) = k in
+  
+  // some *s
+  let k
+    : continuation_elaborator
+        pst.pg ((list_as_vprop pst.remaining_ctxt * preamble.frame) * pst.ss.(pst.solved))
+        g' ((remaining_ctxt' * preamble.frame) * pst.ss.(pst.solved)) =
+    
+    k_elab_equiv k (magic ()) (magic ()) in
+
+  let k_new
+    : continuation_elaborator
+        preamble.g0 (preamble.ctxt * preamble.frame)
+        g' ((remaining_ctxt' * preamble.frame) * pst.ss.(pst.solved)) =
+    k_elab_trans pst.k k in
+  
+  assume (list_as_vprop (vprop_as_list remaining_ctxt') == remaining_ctxt');
+  assume (well_typed_ss pst.ss pst.uvs g');
+
+  { pst with
+    pg = g';
+    remaining_ctxt = vprop_as_list remaining_ctxt';
+    remaining_ctxt_frame_typing = magic ();
+    solved_typing = magic ();  // weakening of pst.solved_typing
+    k = k_new;
+    goals_inv = magic ();  // weakening of pst.goals_inv
+  }
